Hook up the bounded interface, finish proofs

src/BoundedArithmetic/DoubleBounded.v
@@ -1,13 +1,11 @@
 (*** Implementing Large Bounded Arithmetic via pairs *)
-Require Import Coq.ZArith.ZArith Coq.Lists.List.
+Require Import Coq.ZArith.ZArith.
 Require Import Crypto.BoundedArithmetic.Interface.
-Require Import Crypto.BaseSystem.
-Require Import Crypto.BaseSystemProofs.
 Require Import Crypto.ModularArithmetic.Pow2Base.
-Require Import Crypto.Util.ZUtil.
+Require Import Crypto.Util.Tuple.
+Require Import Crypto.Util.ListUtil.
 Require Import Crypto.Util.Notations.
 
-Import ListNotations.
 Local Open Scope list_scope.
 Local Open Scope nat_scope.
 Local Open Scope Z_scope.
@@ -17,6 +15,17 @@ Local Coercion Z.of_nat : nat >-> Z.
 Local Notation eta x := (fst x, snd x).
 
 Section generic_constructions.
+  Section decode.
+    Context {n W} {decode : decoder n W}.
+    Section with_k.
+      Context {k : nat}.
+      Let limb_widths := repeat n k.
+      (** The list is low to high; the tuple is low to high *)
+      Local Instance tuple_decoder : decoder (k * n) (tuple W k)
+        := { decode w := BaseSystem.decode (base_from_limb_widths limb_widths) (List.map decode (List.rev (Tuple.to_list _ w))) }.
+    End with_k.
+  End decode.
+
   Definition ripple_carry {T} (f : T -> T -> bool -> bool * T)
              (xs ys : list T) (carry : bool) : bool * list T
     := List.fold_right
@@ -27,17 +36,91 @@ Section generic_constructions.
          (carry, nil)
          (List.combine xs ys).
 
+  (** tuple is high to low ([to_list] reverses) *)
+  Fixpoint ripple_carry_tuple' {T} (f : T -> T -> bool -> bool * T) k
+    : forall (xs ys : tuple' T k) (carry : bool), bool * tuple' T k
+    := match k return forall (xs ys : tuple' T k) (carry : bool), bool * tuple' T k with
+       | O => f
+       | S k' => fun xss yss carry => let '(xs, x) := eta xss in
+                                      let '(ys, y) := eta yss in
+                                      let '(carry, zs) := eta (@ripple_carry_tuple' _ f k' xs ys carry) in
+                                      let '(carry, z) := eta (f x y carry) in
+                                      (carry, (zs, z))
+       end.
+
+  Definition ripple_carry_tuple {T} (f : T -> T -> bool -> bool * T) k
+    : forall (xs ys : tuple T k) (carry : bool), bool * tuple T k
+    := match k return forall (xs ys : tuple T k) (carry : bool), bool * tuple T k with
+       | O => fun xs ys carry => (carry, tt)
+       | S k' => ripple_carry_tuple' f k'
+       end.
+
   Section ripple_carry_adc.
     Context {n W} {decode : decoder n W} (adc : add_with_carry W).
 
-    Global Instance ripple_carry_add_with_carry : add_with_carry (list W)
-      := {| Interface.adc := ripple_carry adc |}.
-    (*
-    Global Instance ripple_carry_is_add_with_carry {is_adc : is_add_with_carry adc}
-      : is_add_with_carry ripple_carry_add_with_carry.*)
+    Global Instance ripple_carry_adc {k} : add_with_carry (tuple W k)
+      := {| Interface.adc := ripple_carry_tuple adc k |}.
   End ripple_carry_adc.
 
   (* TODO: Would it made sense to make generic-width shift operations here? *)
 
-  (* FUTURE: here go proofs about [ripple_carry] with [f] that satisfies [is_add_with_carry] *)
+  Section tuple2.
+    Section spread_left.
+      Context (n : Z) {W}
+              {ldi : load_immediate W}
+              {shl : shift_left_immediate W}
+              {shr : shift_right_immediate W}.
+
+      Definition spread_left_from_shift (r : W) (count : Z) : tuple W 2
+        := (shl r count, if count =? 0 then ldi 0 else shr r (n - count)).
+
+      (** Require a [decode] instance to aid typeclass search in
+          resolving [n] *)
+      Global Instance sprl_from_shift {decode : decoder n W} : spread_left_immediate W
+        := {| Interface.sprl := spread_left_from_shift |}.
+    End spread_left.
+
+    Section full_from_half.
+      Context {W}
+              {mulhwll : multiply_low_low W}
+              {mulhwhl : multiply_high_low W}
+              {mulhwhh : multiply_high_high W}
+              {adc : add_with_carry W}
+              {shl : shift_left_immediate W}
+              {shr : shift_right_immediate W}.
+
+      Section def.
+        Context (half_n : Z).
+        Definition mul_double (a b : W) : tuple W 2
+          := let out : tuple W 2 := (mulhwll a b, mulhwhh a b) in
+             let tmp             := mulhwhl a b in
+             let '(_, out)   := eta (ripple_carry_adc adc out (shl tmp half_n, shr tmp half_n) false) in
+             let tmp             := mulhwhl b a in
+             let '(_, out)   := eta (ripple_carry_adc adc out (shl tmp half_n, shr tmp half_n) false) in
+             out.
+      End def.
+
+      Section instances.
+        Context {half_n : Z}
+                {ldi : load_immediate W}.
+
+        (** Require a dummy [decoder] for these instances to allow
+            typeclass inference of the [half_n] argument *)
+        Global Instance mul_double_multiply_low_low {decode : decoder (2 * half_n) W}
+          : multiply_low_low (tuple W 2)
+          := {| Interface.mulhwll a b := mul_double half_n (fst a) (fst b) |}.
+        Global Instance mul_double_multiply_high_low {decode : decoder (2 * half_n) W}
+          : multiply_high_low (tuple W 2)
+          := {| Interface.mulhwhl a b := mul_double half_n (snd a) (fst b) |}.
+        Global Instance mul_double_multiply_high_high {decode : decoder (2 * half_n) W}
+          : multiply_high_high (tuple W 2)
+          := {| Interface.mulhwhh a b := mul_double half_n (snd a) (snd b) |}.
+      End instances.
+    End full_from_half.
+  End tuple2.
 End generic_constructions.
+
+Global Arguments tuple_decoder : simpl never.
+
+Hint Resolve (fun n W decode => (@tuple_decoder n W decode 2 : decoder (2 * n) (tuple W 2))) : typeclass_instances.
+Hint Extern 3 (decoder _ (tuple ?W ?k)) => let kv := (eval simpl in (Z.of_nat k)) in apply (fun n decode => (@tuple_decoder n W decode k : decoder (kv * n) (tuple W k))) : typeclass_instances.
