src/BoundedArithmetic/Interface.v
@@ -53,17 +53,31 @@ Section InstructionGallery.
     decode_shift_left_immediate :
       forall r count, 0 <= count < n -> decode (shl r count) = (decode r << count) mod 2^n.
 
-  Record spread_left_immediate := { sprl :> W -> imm -> W * W (* [(high, low)] *) }.
+  Record shift_right_immediate := { shr :> W -> imm -> W }.
+
+  Class is_shift_right_immediate (shr : shift_right_immediate) :=
+    decode_shift_right_immediate :
+      forall r count, 0 <= count < n -> decode (shr r count) = (decode r >> count).
+
+  Record spread_left_immediate := { sprl :> W -> imm -> W * W (* [(low, high)] *) }.
 
   Class is_spread_left_immediate (sprl : spread_left_immediate) :=
     {
       decode_fst_spread_left_immediate : forall r count,
-        0 <= count < n
-        -> decode (fst (sprl r count)) = (decode r << count) >> n;
-      decode_snd_spread_left_immediate : forall r count,
           0 <= count < n
-          -> decode (snd (sprl r count)) = (decode r << count) mod 2^n
+          -> decode (fst (sprl r count)) = (decode r << count) mod 2^n;
+      decode_snd_spread_left_immediate : forall r count,
+        0 <= count < n
+        -> decode (snd (sprl r count)) = (decode r << count) >> n;
+
     }.
+
+  Definition Build_is_spread_left_immediate' (sprl : spread_left_immediate)
+             (pf : forall r count, 0 <= count < n
+                                   -> decode (fst (sprl r count)) = (decode r << count) mod 2^n
+                                      /\ decode (snd (sprl r count)) = (decode r << count) >> n)
+    := {| decode_fst_spread_left_immediate r count H := proj1 (pf r count H);
+          decode_snd_spread_left_immediate r count H := proj2 (pf r count H) |}.
 
   Record mask_keep_low := { mkl :> W -> imm -> W }.
 
@@ -81,6 +95,11 @@ Section InstructionGallery.
       decode_snd_add_with_carry : forall x y c, decode (snd (adc x y c)) = (decode x + decode y + bit c) mod (2^n)
     }.
 
+  Definition Build_is_add_with_carry' (adc : add_with_carry)
+             (pf : forall x y c, bit (fst (adc x y c)) = (decode x + decode y + bit c) >> n /\ decode (snd (adc x y c)) = (decode x + decode y + bit c) mod (2^n))
+    := {| bit_fst_add_with_carry x y c := proj1 (pf x y c);
+          decode_snd_add_with_carry x y c := proj2 (pf x y c) |}.
+
   Record sub_with_carry := { subc :> W -> W -> bool -> bool * W }.
 
   Class is_sub_with_carry (subc:W->W->bool->bool*W) :=
@@ -88,6 +107,11 @@ Section InstructionGallery.
       fst_sub_with_carry : forall x y c, fst (subc x y c) = ((decode x - decode y - bit c) <? 0);
       decode_snd_sub_with_carry : forall x y c, decode (snd (subc x y c)) = (decode x - decode y - bit c) mod 2^n
     }.
+
+  Definition Build_is_sub_with_carry' (subc : sub_with_carry)
+             (pf : forall x y c, fst (subc x y c) = ((decode x - decode y - bit c) <? 0) /\ decode (snd (subc x y c)) = (decode x - decode y - bit c) mod 2^n)
+    := {| fst_sub_with_carry x y c := proj1 (pf x y c);
+          decode_snd_sub_with_carry x y c := proj2 (pf x y c) |}.
 
   Record multiply := { mul :> W -> W -> W }.
 
@@ -118,12 +142,15 @@ Section InstructionGallery.
 
   Class is_add_modulo (addm : add_modulo) :=
     decode_add_modulo : forall x y modulus,
-      decode (addm x y modulus) = (decode x + decode y) mod (decode modulus).
+      decode (addm x y modulus) = (if (decode x + decode y) <? decode modulus
+                                   then (decode x + decode y)
+                                   else (decode x + decode y) - decode modulus)%Z.
 End InstructionGallery.
 
 Global Arguments load_immediate : clear implicits.
 Global Arguments shift_right_doubleword_immediate : clear implicits.
 Global Arguments shift_left_immediate : clear implicits.
+Global Arguments shift_right_immediate : clear implicits.
 Global Arguments spread_left_immediate : clear implicits.
 Global Arguments mask_keep_low : clear implicits.
 Global Arguments add_with_carry : clear implicits.
@@ -137,6 +164,7 @@ Global Arguments add_modulo : clear implicits.
 Global Arguments ldi {_ _} _.
 Global Arguments shrd {_ _} _ _ _.
 Global Arguments shl {_ _} _ _.
+Global Arguments shr {_ _} _ _.
 Global Arguments sprl {_ _} _ _.
 Global Arguments mkl {_ _} _ _.
 Global Arguments adc {_ _} _ _ _.
@@ -151,6 +179,7 @@ Global Arguments addm {_ _} _ _ _.
 Existing Class load_immediate.
 Existing Class shift_right_doubleword_immediate.
 Existing Class shift_left_immediate.
+Existing Class shift_right_immediate.
 Existing Class spread_left_immediate.
 Existing Class mask_keep_low.
 Existing Class add_with_carry.
@@ -166,6 +195,7 @@ Global Arguments is_decode {_ _} _.
 Global Arguments is_load_immediate {_ _ _} _.
 Global Arguments is_shift_right_doubleword_immediate {_ _ _} _.
 Global Arguments is_shift_left_immediate {_ _ _} _.
+Global Arguments is_shift_right_immediate {_ _ _} _.
 Global Arguments is_spread_left_immediate {_ _ _} _.
 Global Arguments is_mask_keep_low {_ _ _} _.
 Global Arguments is_add_with_carry {_ _ _} _.
@@ -177,45 +207,91 @@ Global Arguments is_mul_high_high {_ _ _} _ _.
 Global Arguments is_select_conditional {_ _ _} _.
 Global Arguments is_add_modulo {_ _ _} _.
 
-Ltac bounded_sovlver_tac :=
-  solve [ eassumption | typeclasses eauto | omega | auto 6 using decode_range with typeclass_instances omega ].
+Ltac bounded_solver_tac :=
+  solve [ eassumption | typeclasses eauto | omega ].
 
-Hint Rewrite @decode_load_immediate @decode_shift_right_doubleword @decode_shift_left_immediate @decode_fst_spread_left_immediate @decode_snd_spread_left_immediate @decode_mask_keep_low @bit_fst_add_with_carry @decode_snd_add_with_carry @fst_sub_with_carry @decode_snd_sub_with_carry @decode_mul @decode_mul_low_low @decode_mul_high_low @decode_mul_high_high @decode_select_conditional @decode_add_modulo using bounded_sovlver_tac : push_decode.
+Lemma decode_proj n W (dec : W -> Z)
+  : @decode n W {| decode := dec |} = dec.
+Proof. reflexivity. Qed.
 
-Ltac push_decode :=
-  repeat first [ erewrite !decode_load_immediate by bounded_sovlver_tac
-               | erewrite !decode_shift_right_doubleword by bounded_sovlver_tac
-               | erewrite !decode_shift_left_immediate by bounded_sovlver_tac
-               | erewrite !decode_fst_spread_left_immediate by bounded_sovlver_tac
-               | erewrite !decode_snd_spread_left_immediate by bounded_sovlver_tac
-               | erewrite !decode_mask_keep_low by bounded_sovlver_tac
-               | erewrite !bit_fst_add_with_carry by bounded_sovlver_tac
-               | erewrite !decode_snd_add_with_carry by bounded_sovlver_tac
-               | erewrite !fst_sub_with_carry by bounded_sovlver_tac
-               | erewrite !decode_snd_sub_with_carry by bounded_sovlver_tac
-               | erewrite !decode_mul by bounded_sovlver_tac
-               | erewrite !decode_mul_low_low by bounded_sovlver_tac
-               | erewrite !decode_mul_high_low by bounded_sovlver_tac
-               | erewrite !decode_mul_high_high by bounded_sovlver_tac
-               | erewrite !decode_select_conditional by bounded_sovlver_tac
-               | erewrite !decode_add_modulo by bounded_sovlver_tac ].
-Ltac pull_decode :=
-  repeat first [ erewrite <- !decode_load_immediate by bounded_sovlver_tac
-               | erewrite <- !decode_shift_right_doubleword by bounded_sovlver_tac
-               | erewrite <- !decode_shift_left_immediate by bounded_sovlver_tac
-               | erewrite <- !decode_fst_spread_left_immediate by bounded_sovlver_tac
-               | erewrite <- !decode_snd_spread_left_immediate by bounded_sovlver_tac
-               | erewrite <- !decode_mask_keep_low by bounded_sovlver_tac
-               | erewrite <- !bit_fst_add_with_carry by bounded_sovlver_tac
-               | erewrite <- !decode_snd_add_with_carry by bounded_sovlver_tac
-               | erewrite <- !fst_sub_with_carry by bounded_sovlver_tac
-               | erewrite <- !decode_snd_sub_with_carry by bounded_sovlver_tac
-               | erewrite <- !decode_mul by bounded_sovlver_tac
-               | erewrite <- !decode_mul_low_low by bounded_sovlver_tac
-               | erewrite <- !decode_mul_high_low by bounded_sovlver_tac
-               | erewrite <- !decode_mul_high_high by bounded_sovlver_tac
-               | erewrite <- !decode_select_conditional by bounded_sovlver_tac
-               | erewrite <- !decode_add_modulo by bounded_sovlver_tac ].
+Lemma decode_exponent_nonnegative {n W} (decode : decoder n W) {isdecode : is_decode decode}
+      (isinhabited : W)
+  : 0 <= n.
+Proof.
+  pose proof (decode_range isinhabited).
+  assert (0 < 2^n) by omega.
+  destruct (Z_lt_ge_dec n 0) as [H'|]; [ | omega ].
+  assert (2^n = 0) by auto using Z.pow_neg_r.
+  omega.
+Qed.
+
+Hint Rewrite @decode_load_immediate @decode_shift_right_doubleword @decode_shift_left_immediate @decode_shift_right_immediate @decode_fst_spread_left_immediate @decode_snd_spread_left_immediate @decode_mask_keep_low @bit_fst_add_with_carry @decode_snd_add_with_carry @fst_sub_with_carry @decode_snd_sub_with_carry @decode_mul @decode_mul_low_low @decode_mul_high_low @decode_mul_high_high @decode_select_conditional @decode_add_modulo @decode_proj using bounded_solver_tac : push_decode.
+
+Ltac push_decode_step :=
+  first [ rewrite !decode_proj
+        | erewrite !decode_load_immediate by bounded_solver_tac
+        | erewrite !decode_shift_right_doubleword by bounded_solver_tac
+        | erewrite !decode_shift_left_immediate by bounded_solver_tac
+        | erewrite !decode_shift_right_immediate by bounded_solver_tac
+        | erewrite !decode_fst_spread_left_immediate by bounded_solver_tac
+        | erewrite !decode_snd_spread_left_immediate by bounded_solver_tac
+        | erewrite !decode_mask_keep_low by bounded_solver_tac
+        | erewrite !bit_fst_add_with_carry by bounded_solver_tac
+        | erewrite !decode_snd_add_with_carry by bounded_solver_tac
+        | erewrite !fst_sub_with_carry by bounded_solver_tac
+        | erewrite !decode_snd_sub_with_carry by bounded_solver_tac
+        | erewrite !decode_mul by bounded_solver_tac
+        | erewrite !decode_mul_low_low by bounded_solver_tac
+        | erewrite !decode_mul_high_low by bounded_solver_tac
+        | erewrite !decode_mul_high_high by bounded_solver_tac
+        | erewrite !decode_select_conditional by bounded_solver_tac
+        | erewrite !decode_add_modulo by bounded_solver_tac ].
+Ltac pull_decode_step :=
+  first [ erewrite <- !decode_load_immediate by bounded_solver_tac
+        | erewrite <- !decode_shift_right_doubleword by bounded_solver_tac
+        | erewrite <- !decode_shift_left_immediate by bounded_solver_tac
+        | erewrite <- !decode_shift_right_immediate by bounded_solver_tac
+        | erewrite <- !decode_fst_spread_left_immediate by bounded_solver_tac
+        | erewrite <- !decode_snd_spread_left_immediate by bounded_solver_tac
+        | erewrite <- !decode_mask_keep_low by bounded_solver_tac
+        | erewrite <- !bit_fst_add_with_carry by bounded_solver_tac
+        | erewrite <- !decode_snd_add_with_carry by bounded_solver_tac
+        | erewrite <- !fst_sub_with_carry by bounded_solver_tac
+        | erewrite <- !decode_snd_sub_with_carry by bounded_solver_tac
+        | erewrite <- !decode_mul by bounded_solver_tac
+        | erewrite <- !decode_mul_low_low by bounded_solver_tac
+        | erewrite <- !decode_mul_high_low by bounded_solver_tac
+        | erewrite <- !decode_mul_high_high by bounded_solver_tac
+        | erewrite <- !decode_select_conditional by bounded_solver_tac
+        | erewrite <- !decode_add_modulo by bounded_solver_tac ].
+Ltac push_decode := repeat push_decode_step.
+Ltac pull_decode := repeat pull_decode_step.
+
+(* We take special care to handle the case where the decoder is
+   syntactically different but the decoded expression is judgmentally
+   the same; we don't want to split apart variables that should be the
+   same. *)
+Ltac set_decode_step check :=
+  match goal with
+  | [ |- context G[@Interface.decode ?n ?W ?dr ?w] ]
+    => check w;
+      first [ match goal with
+              | [ d := @Interface.decode _ _ _ w |- _ ]
+                => change (@Interface.decode n W dr w) with d
+              end
+            | generalize (@decode_range n W dr _ w);
+              let d := fresh "d" in
+              set (d := @Interface.decode n W dr w);
+              intro ]
+  end.
+Ltac set_decode check := repeat set_decode_step check.
+Ltac clearbody_decode :=
+  repeat match goal with
+         | [ H := @Interface.decode _ _ _ _ |- _ ] => clearbody H
+         end.
+Ltac generalize_decode_by check := set_decode check; clearbody_decode.
+Ltac generalize_decode := generalize_decode_by ltac:(fun w => idtac).
+Ltac generalize_decode_var := generalize_decode_by ltac:(fun w => is_var w).
 
 Module fancy_machine.
   Local Notation imm := Z (only parsing).
@@ -227,6 +303,7 @@ Module fancy_machine.
       ldi :> load_immediate W;
       shrd :> shift_right_doubleword_immediate W;
       shl :> shift_left_immediate W;
+      shr :> shift_right_immediate W;
       mkl :> mask_keep_low W;
       adc :> add_with_carry W;
       subc :> sub_with_carry W;
@@ -243,6 +320,7 @@ Module fancy_machine.
       load_immediate :> is_load_immediate ldi;
       shift_right_doubleword_immediate :> is_shift_right_doubleword_immediate shrd;
       shift_left_immediate :> is_shift_left_immediate shl;
+      shift_right_immediate :> is_shift_right_immediate shr;
       mask_keep_low :> is_mask_keep_low mkl;
       add_with_carry :> is_add_with_carry adc;
       sub_with_carry :> is_sub_with_carry subc;
