src/BoundedArithmetic/ArchitectureToZLike.v
@@ -3,123 +3,28 @@ Require Import Coq.ZArith.ZArith.
 Require Import Crypto.BoundedArithmetic.Interface.
 Require Import Crypto.BoundedArithmetic.DoubleBounded.
 Require Import Crypto.ModularArithmetic.ZBounded.
-Require Import Coq.Lists.List.
-Import ListNotations.
+Require Import Crypto.Util.Tuple.
 
-Local Open Scope nat_scope.
 Local Open Scope Z_scope.
-Local Open Scope type_scope.
-
-Local Coercion Z.of_nat : nat >-> Z.
 
 Section fancy_machine_p256_montgomery_foundation.
   Context {n_over_two : Z}.
-  Local Notation n := (2 * n_over_two)%Z.
+  Local Notation n := (2 * n_over_two).
   Context (ops : fancy_machine.instructions n) (modulus : Z).
-
-  Definition two_list_to_tuple {A B} (x : A * list B)
-    := match x return match x with
-                      | (a, [b0; b1]) => A * (B * B)
-                      | _ => True
-                      end
-       with
-       | (a, [b0; b1]) => (a, (b0, b1))
-       | _ => I
-       end.
-(*
-  (* make all machine-specific constructions here, preferrably as
-  thing wrappers around generic constructions *)
-    Local Instance DoubleArchitectureBoundedOps : ArchitectureBoundedOps (2 * n)%nat
-      := { BoundedType := BoundedType * BoundedType (* [(high, low)] *);
-           decode high_low := (decode (fst high_low) * 2^n + decode (snd high_low))%Z;
-           encode z := (encode (z / 2^n), encode (z mod 2^n));
-           ShiftRight a high_low
-           := let '(high, low) := eta high_low in
-              if n <=? a then
-                (ShiftRight (a - n)%nat (encode 0, fst high), ShiftRight (a - n)%nat high)
-              else
-                (ShiftRight a (snd high, fst low), ShiftRight a low);
-           ShiftLeft a high_low
-           := let '(high, low) := eta high_low in
-              if 2 * n <=? a then
-                let '(high0, low) := eta (ShiftLeft (a - 2 * n)%nat low) in
-                let '(high_high, high1) := eta (ShiftLeft (a - 2 * n)%nat high) in
-                ((snd (CarryAdd false high0 high1), low), (encode 0, encode 0))
-              else if n <=? a then
-                     let '(high0, low) := eta (ShiftLeft (a - n)%nat low) in
-                     let '(high_high, high1) := eta (ShiftLeft (a - n)%nat high) in
-                     ((high_high, snd (CarryAdd false high0 high1)), (low, encode 0))
-                   else
-                     let '(high0, low) := eta (ShiftLeft a low) in
-                     let '(high_high, high1) := eta (ShiftLeft a high) in
-                     ((encode 0, high_high), (snd (CarryAdd false high0 high1), low));
-           Mod2Pow a high_low
-           := let '(high, low) := (fst high_low, snd high_low) in
-              (Mod2Pow (a - n)%nat high, Mod2Pow a low);
-           CarryAdd carry x_high_low y_high_low
-           := let '(xhigh, xlow) := eta x_high_low in
-              let '(yhigh, ylow) := eta y_high_low in
-              two_list_to_tuple (ripple_carry CarryAdd carry [xhigh; xlow] [yhigh; ylow]);
-           CarrySub carry x_high_low y_high_low
-           := let '(xhigh, xlow) := eta x_high_low in
-              let '(yhigh, ylow) := eta y_high_low in
-              two_list_to_tuple (ripple_carry CarrySub carry [xhigh; xlow] [yhigh; ylow]) }.
-
-    Definition BoundedOfHalfBounded (x : @BoundedHalfType (2 * n)%nat _) : @BoundedType n _
-      := match x with
-         | UpperHalf x => fst x
-         | LowerHalf x => snd x
-         end.
-
-    Local Instance DoubleArchitectureBoundedHalfWidthMulOpsOfFullMulOps
-          {base_mops : ArchitectureBoundedFullMulOps n}
-      : ArchitectureBoundedHalfWidthMulOps (2 * n)%nat :=
-      { HalfWidthMul a b
-        := Mul (BoundedOfHalfBounded a) (BoundedOfHalfBounded b) }.
-  End single.
-
-  Local Existing Instance DoubleArchitectureBoundedOps.
-
-  Section full_from_half.
-    Context (n : size) {base_ops : ArchitectureBoundedOps (2 * n)%nat}.
-
-    Local Infix "*" := HalfWidthMul.
-
-    Local Instance DoubleArchitectureBoundedFullMulOpsOfHalfWidthMulOps
-          {base_mops : ArchitectureBoundedHalfWidthMulOps (2 * n)%nat}
-      : ArchitectureBoundedFullMulOps (2 * n)%nat :=
-      { Mul a b
-        := let '(a1, a0) := (UpperHalf a, LowerHalf a) in
-           let '(b1, b0) := (UpperHalf b, LowerHalf b) in
-           let out := a0 * b0 in
-           let outHigh := a1 * b1 in
-           let tmp := a1 * b0 in
-           let '(carry, out) := eta (CarryAdd false out (snd (ShiftLeft n tmp))) in
-           let '(_, outHigh) := eta (CarryAdd carry outHigh (ShiftRight n (encode 0, tmp))) in
-           let tmp := a0 * b1 in
-           let '(carry, out) := eta (CarryAdd false out (snd (ShiftLeft n tmp))) in
-           let '(_, outHigh) := eta (CarryAdd carry outHigh (ShiftRight n (encode 0, tmp))) in
-           (outHigh, out) }.
-  End full_from_half.
-
-  Local Existing Instance DoubleArchitectureBoundedFullMulOpsOfHalfWidthMulOps.
-*)
-  Axiom admit : forall {T}, T.
 
   Global Instance ZLikeOps_of_ArchitectureBoundedOps (smaller_bound_exp : Z)
     : ZLikeOps (2^n) (2^smaller_bound_exp) modulus :=
-    { LargeT := fancy_machine.W * fancy_machine.W;
+    { LargeT := tuple fancy_machine.W 2;
       SmallT := fancy_machine.W;
       modulus_digits := ldi modulus;
-      decode_large := _;
+      decode_large := decode;
       decode_small := decode;
-      Mod_SmallBound v := snd v;
-      DivBy_SmallBound v := fst v;
-      DivBy_SmallerBound v := shrd (fst v) (snd v) smaller_bound_exp;
-      Mul x y := _  (*mulhwll (ldi 0, x) (ldi 0, y)*);
-      CarryAdd x y := _ (*adc x y false*);
+      Mod_SmallBound v := fst v;
+      DivBy_SmallBound v := snd v;
+      DivBy_SmallerBound v := shrd (snd v) (fst v) smaller_bound_exp;
+      Mul x y := mulhwll (W := tuple _ 2) (sprl x 0) (sprl y 0);
+      CarryAdd x y := adc x y false;
       CarrySubSmall x y := subc x y false;
-      ConditionalSubtract b x := let v := selc b (ldi 0) (ldi modulus) in snd (subc x v false);
+      ConditionalSubtract b x := let v := selc b (ldi modulus) (ldi 0) in snd (subc x v false);
       ConditionalSubtractModulus y := addm y (ldi 0) (ldi modulus) }.
-  Abort.
 End fancy_machine_p256_montgomery_foundation.
