src/BoundedArithmetic/ArchitectureToZLikeProofs.v
@@ -1,0 +1,109 @@
+(*** Proving ℤ-Like via Architecture *)
+Require Import Coq.ZArith.ZArith.
+Require Import Crypto.BoundedArithmetic.Interface.
+Require Import Crypto.BoundedArithmetic.DoubleBounded.
+Require Import Crypto.BoundedArithmetic.DoubleBoundedProofs.
+Require Import Crypto.BoundedArithmetic.ArchitectureToZLike.
+Require Import Crypto.ModularArithmetic.ZBounded.
+Require Import Crypto.Util.Tuple.
+Require Import Crypto.Util.ZUtil Crypto.Util.Tactics.
+
+Local Open Scope nat_scope.
+Local Open Scope Z_scope.
+Local Open Scope type_scope.
+
+Local Coercion Z.of_nat : nat >-> Z.
+
+Section fancy_machine_p256_montgomery_foundation.
+  Context {n_over_two : Z}.
+  Local Notation n := (2 * n_over_two)%Z.
+  Context (ops : fancy_machine.instructions n) (modulus : Z).
+
+  Local Arguments Z.mul !_ !_.
+  Local Arguments BaseSystem.decode !_ !_ / .
+  Local Arguments BaseSystem.accumulate / .
+  Local Arguments BaseSystem.decode' !_ !_ / .
+
+  Local Ltac introduce_t_step :=
+    match goal with
+    | [ |- forall x : bool, _ ] => intros [|]
+    | [ |- True -> _ ] => intros _
+    | [ |- _ <= _ < _ -> _ ] => intro
+    | _ => let x := fresh "x" in
+           intro x;
+           try pose proof (decode_range (fst x));
+           try pose proof (decode_range (snd x));
+           pose proof (decode_range x)
+    end.
+  Local Ltac unfolder_t :=
+    progress unfold LargeT, SmallT, modulus_digits, decode_large, decode_small, Mod_SmallBound, DivBy_SmallBound, DivBy_SmallerBound, Mul, CarryAdd, CarrySubSmall, ConditionalSubtract, ConditionalSubtractModulus, ZLikeOps_of_ArchitectureBoundedOps in *.
+  Local Ltac saturate_context_step :=
+    match goal with
+    | _ => unique assert (0 <= 2 * n_over_two) by solve [ eauto using decode_exponent_nonnegative with typeclass_instances | omega ]
+    | _ => unique assert (0 <= n_over_two) by solve [ eauto using decode_exponent_nonnegative with typeclass_instances | omega ]
+    | _ => unique assert (0 <= 2 * (2 * n_over_two)) by (eauto using decode_exponent_nonnegative with typeclass_instances)
+    end.
+  Local Ltac pre_t :=
+    repeat first [ tauto
+                 | introduce_t_step
+                 | unfolder_t
+                 | saturate_context_step ].
+  Local Ltac post_t_step :=
+    match goal with
+    | _ => tauto
+    | _ => progress autorewrite with zsimplify_const in *
+    | _ => progress push_decode
+    | _ => progress autorewrite with push_Zpow in *
+    | _ => progress Z.rewrite_mod_small
+    | [ |- fst ?x = (?a <=? ?b) :> bool ]
+      => cut (((if fst x then 1 else 0) = (if a <=? b then 1 else 0))%Z);
+         [ destruct (fst x), (a <=? b); intro; congruence | ]
+    | [ |- appcontext[let (a, b) := ?x in _] ]
+      => rewrite (surjective_pairing x); simplify_projections
+    | _ => progress autorewrite with Zshift_to_pow in *
+    | _ => progress autorewrite with simpl_tuple_decoder in *
+    | _ => progress autorewrite with zsimplify
+    | [ |- _ / ?y = _ / ?y ] => apply f_equal2; omega
+    | [ |- _ / _ = if _ then _ else _ ] => apply Z.div_between_0_if; auto with zarith omega
+    end.
+  Local Ltac post_t := repeat post_t_step.
+  Local Ltac t := pre_t; post_t.
+
+  Global Instance ZLikeProperties_of_ArchitectureBoundedOps
+         {arith : fancy_machine.arithmetic ops}
+         (modulus_in_range : 0 <= modulus < 2^n)
+         (smaller_bound_exp : Z)
+         (smaller_bound_smaller : 0 <= smaller_bound_exp < n)
+    : ZLikeProperties (ZLikeOps_of_ArchitectureBoundedOps ops modulus smaller_bound_exp)
+    := { large_valid v := True;
+         medium_valid v := 0 <= decode_large v < 2^n * 2^smaller_bound_exp;
+         small_valid v := True }.
+  Proof.
+    (* In 8.5: *)
+    (* par:t. *)
+    { abstract t. }
+    { abstract t. }
+    { abstract t. }
+    { abstract t. }
+    { abstract t. }
+    { abstract t. }
+    { abstract t. }
+    { abstract t. }
+    { abstract t. }
+    { abstract t. }
+    { abstract t. }
+    { abstract t. }
+    { abstract t. }
+    { abstract t. }
+    { abstract t. }
+    { abstract t. }
+    { abstract t. }
+    { abstract t. }
+    { abstract t. }
+    { abstract t. }
+    { abstract t. }
+    { abstract t. }
+    { abstract t. }
+    { abstract t. }
+  Defined.
+End fancy_machine_p256_montgomery_foundation.
